

Proof 1

$$b = a^T Y \quad E[b] = a^T X \beta = \beta \Rightarrow a^T X = I$$

$$\mathcal{L} = \sigma^2 a^T a - (a^T X - I) \lambda$$

$$\frac{\partial \mathcal{L}}{\partial a} = 0 \Rightarrow a = \frac{X \lambda}{2 \sigma^2} \quad \frac{\partial \mathcal{L}}{\partial \lambda} = 0 \Rightarrow a^T X = I$$

$$\frac{\lambda^T X^T X}{2 \sigma^2} = I \Rightarrow \lambda^T = 2 \sigma^2 (X^T X)^{-1}$$

$$a = X (X^T X)^{-T} \Rightarrow b = (X^T X)^{-1} X^T Y$$

Proof 2

$$e = (I_n - H) Y \quad MSE = \frac{SSE}{n - p}$$

$$E[Y^T (I_n - H) Y] = E[(X \beta + \varepsilon)^T (I_n - H) (X \beta + \varepsilon)]$$

$$\beta^T X^T (I_n - H) X \beta + 2 \beta^T X^T (I_n - H) E[\varepsilon] + E[\varepsilon^T (I_n - H) \varepsilon]$$

$$\beta^T X^T (X - X (X^T X)^{-1} X^T X) \beta + 0 + tr((I_n - H) \sigma^2) + E[\varepsilon]^T (I_n - H) E[\varepsilon]$$

$$\sigma^2 (tr(I_n) - tr(H))$$

$$\sigma^2 (tr(I_n) - tr(X (X^T X)^{-1} X^T))$$

$$\sigma^2 (tr(I_n) - tr(I_p))$$

$$\sigma^2 (n - p)$$

Distribution	Notes	Lower	Upper
$\frac{(n-1)s^2}{\sigma^2} \sim \chi^2_{n-1}$	$s \rightarrow MSE \Rightarrow n-1 \rightarrow n-p$	$\frac{(n-1)s^2}{\chi^2_{n-1,1-\alpha/2}}$	$\frac{(n-1)s^2}{\chi^2_{n-1,\alpha/2}}$
$\frac{\bar{Y}-\mu}{s/\sqrt{n}} \sim t_{n-1}$	$\bar{Y} \sim N(\mu, \frac{\sigma^2}{n})$	$\bar{Y} - t_{n-1,1-\alpha/2} \frac{s}{\sqrt{n}}$	$\bar{Y} + t_{n-1,1-\alpha/2} \frac{s}{\sqrt{n}}$
$\frac{\bar{Y}_1 - \bar{Y}_2 - (\mu_1 - \mu_2)}{s_p \sqrt{\frac{1}{n_1} + \frac{1}{n_2}}} \sim t_{n_1+n_2-2}$	$\sigma_1^2 = \sigma_2^2$	$\bar{Y}_1 - \bar{Y}_2 - t_{n_1+n_2-2,1-\alpha/2} s_p \sqrt{\frac{1}{n_1} + \frac{1}{n_2}}$	$\bar{Y}_1 - \bar{Y}_2 + t_{n_1+n_2-2,1-\alpha/2} s_p \sqrt{\frac{1}{n_1} + \frac{1}{n_2}}$
$\frac{\bar{Y}_1 - \bar{Y}_2 - (\mu_1 - \mu_2)}{\sqrt{\frac{s_1^2}{n_1} + \frac{s_2^2}{n_2}}} \sim t_{df}$	$df = \left(\frac{s_1^2}{n_1} + \frac{s_2^2}{n_2} \right)^2 \bigg/ \left(\frac{s_1^4}{n_1^2(n_1-1)} + \frac{s_2^4}{n_2^2(n_2-1)} \right)$	$\bar{Y}_1 - \bar{Y}_2 - t_{df,1-\alpha/2} \sqrt{\frac{s_1^2}{n_1} + \frac{s_2^2}{n_2}}$	$\bar{Y}_1 - \bar{Y}_2 + t_{df,1-\alpha/2} \sqrt{\frac{s_1^2}{n_1} + \frac{s_2^2}{n_2}}$
$\frac{s_1^2}{s_2^2} \frac{\sigma_2^2}{\sigma_1^2} \sim F_{n_1-1, n_2-1}$	$\sigma_1^2 = \sigma_2^2$ under H_0	$\frac{s_1^2}{s_2^2} / F_{n_1-1, n_2-1, 1-\alpha/2},$	$\frac{s_1^2}{s_2^2} / F_{n_1-1, n_2-1, \alpha/2}$
$z' = \frac{1}{2} \log \left(\frac{1+r}{1-r} \right)$ Need CLT, $\hat{\rho} = r$	Pearson $\rho = 0 \Rightarrow \beta_1 = 0$ under $H_0, r = \frac{e^{2z}-1}{e^{2z}+1}$	$z' - Z_{1-\alpha/2} \sqrt{\frac{1}{n-3}}$	$z' + Z_{1-\alpha/2} \sqrt{\frac{1}{n-3}}$
$\frac{\bar{d}_1 - \bar{d}_2}{s \sqrt{\frac{1}{n_1} + \frac{1}{n_2}}} \sim t_{n-2}$ Under H_0 need CLT	BF $s^2 = \frac{(\sum_1^{n_1} (d_{i1} - \bar{d}_1) + \sum_1^{n_2} (d_{i2} - \bar{d}_2))}{n-2}$ $d_{ij} = e_{ij} - med(e_j) $	$\bar{d}_1 - \bar{d}_2 - t_{n-2,1-\alpha/2} s \sqrt{\frac{1}{n_1} + \frac{1}{n_2}}$	$\bar{d}_1 - \bar{d}_2 + t_{n-2,1-\alpha/2} s \sqrt{\frac{1}{n_1} + \frac{1}{n_2}}$
$\frac{SSR^*/2}{(SSE/n)^2} \sim \chi_1^2$ Under H_0	BP $\varepsilon_i \sim N(0, \sigma_i^2) \quad \log \sigma_i^2 = \gamma_0 + \gamma_1 x_i$ $H_0: \gamma_1 = 0 \quad SSR^*$ from $lm(e^2 \sim x)$		
$\frac{b_k - \beta_k}{s(b_k)} \sim t_{n-p}$	$s^2(\mathbf{b}) = MSE(X^T X)^{-1}$	$b_k - t_{n-p,1-\alpha/2} s(b_k)$	$b_k + t_{n-p,1-\alpha/2} s(b_k)$
$\frac{\hat{Y}_h - Y_h}{s(\hat{Y}_h)} \sim t_{n-p}$	$s^2(\hat{Y}_h) = MSE X_h^T (X^T X)^{-1} X_h$	$\hat{Y}_h - t_{n-p,1-\alpha/2} s(\hat{Y}_h)$	$\hat{Y}_h + t_{n-p,1-\alpha/2} s(\hat{Y}_h)$
$\frac{\hat{Y}_{h,new} - Y_{h,new}}{s(\hat{Y}_{h,new})} \sim t_{n-p}$	$s^2(\hat{Y}_{h,new}) = MSE(1 + X_h^T (X^T X)^{-1} X_h)$	$\hat{Y}_{h,new} - t_{n-p,1-\alpha/2} s(\hat{Y}_{h,new})$	$\hat{Y}_{h,new} + t_{n-p,1-\alpha/2} s(\hat{Y}_{h,new})$

Source	SS	df	MS	F-value	Pr>F
Regression	SSR	$p-1$	$MSR = \frac{SSR}{p-1}$	$F^* = \frac{MSR}{MSE}$	p-value
Error	SSE	$n-p$	$MSE = \frac{SSE}{n-p}$		
Total	SSTO	$n-1$			

$$H_0 : \beta_1 = \cdots = \beta_{p-1} = 0$$

$$H_a : \text{Not all } \beta_k \text{'s are zero}$$

$$F^* \sim F_{p-1, n-p}$$

Model	Hypothesis	F-Statistic
$Y_i = \beta_0 + \beta_1 x_1 + \varepsilon_i$	$H_0 : \beta_1 = 0$	$\frac{SSR(x_1)}{MSE(x_1)}$
$Y_i = \beta_0 + \beta_1 x_1 + \beta_2 x_2 + \varepsilon_i$	$H_0 : \beta_2 = 0$	$\frac{SSR(x_2 x_1)}{MSE(x_1, x_2)}$
$Y_i = \beta_0 + \beta_1 x_1 + \beta_2 x_2 + \beta_3 x_3 + \varepsilon_i$	$H_0 : \beta_3 = 0$	$\frac{SSR(x_3 x_1, x_2)}{MSE(x_1, x_2, x_3)}$

$$SSR(F) = SSR(x_1, x_2, x_3) = SSR(x_1) + SSR(x_2|x_1) + SSR(x_3|x_1, x_2)$$

How much total variation is reduced when adding the other covariates

Can we drop q predictors from the model?

$$F^* = \frac{(SSE(R) - SSE(F))/q}{SSE(F)/(n-p)} = \frac{SSR(\{x_i\}_{i=j+1}^k | \{x_i\}_{i=1}^j)/q}{SSE(F)/(n-p)} \sim F_{q, n-p}$$

$$H_0 : \beta_{i_1} = \cdots = \beta_{i_q} = 0$$

$$H_a : \text{Not all are 0}$$

ANOVA	df	Sun Sq	Mean Sq	F-Statistic	p-value
x_1	1	$SSR(x_1)$	$SSR(x_1)$	$\frac{SSR(x_1)}{MSE(F)} \sim F_{1, n-2}$	p-value(x_1)
x_2	1	$SSR(x_2 x_1)$	$SSR(x_2 x_1)$	$\frac{SSR(x_2 x_1)}{MSE(F)} \sim F_{1, n-3}$	p-value($x_2 x_1$)
\vdots	\vdots	\vdots	\vdots	\vdots	
x_{p-1}	1	$SSR(F)$	$SSR(F)$	$\frac{SSR(F)}{MSE(F)} \sim F_{1, n-p}$	p-value(F)
Residuals	$n-p$	$SSE(F)$	$MSE(F) = \frac{SSE(F)}{n-p}$		(p-value(F) is same at t p-value(F))

$$SSTO = \sum Sum Sq$$

$$(SSE(R) - SSE(F)) =$$

$$SSR(\{x_i\}_{i=j+1}^k | \{x_i\}_{i=1}^j)$$